Mbse.lean
@@ -4,5 +4,6 @@ import Mbse.Wymore
 import Mbse.Notation
 import Mbse.CombinationalWymore
 import Mbse.DPDAWymore
+import Mbse.GeneralizedWymore
 
 
